src/ecSection.ml
@@ -1353,8 +1353,8 @@ let add_item_ (item : theory_item) (scenv:scenv) =
     | Th_reduction r     -> EcEnv.Reduction.add r env
     | Th_bitstring bs    -> EcEnv.Circ.bind_bitstring env bs
     | Th_bsarray   ba    -> EcEnv.Circ.bind_bsarray env ba
+    | Th_qfabvop   op    -> EcEnv.Circ.bind_qfabvop env op
     | Th_circuit (o, c)  -> EcEnv.Circ.bind_circuit env o c
-    | Th_qfabvop (o, c)  -> EcEnv.Circ.bind_qfabvop env o c
     | _                  -> assert false
   in
   { scenv with
