theories/datatypes/QFABV.ec
@@ -14,7 +14,7 @@ abstract theory BV.
   op oflist : bool list -> bv.
 
   op get (b: bv) (n: int) : bool = 
-	List.nth false (tolist b) n.
+    List.nth false (tolist b) n.
 
   op toint (b: bv) : int = 
     bs2int (tolist b).
@@ -28,15 +28,71 @@ abstract theory BV.
     op bvadd : bv -> bv -> bv.
 
     axiom bvaddP (bv1 bv2 : bv) :
-     toint (bvadd bv1 bv2) = (toint bv1 + toint bv2) %% 2^size.
+      toint (bvadd bv1 bv2) = (toint bv1 + toint bv2) %% 2^size.
   end BVAdd.
 
   abstract theory BVSub.
     op bvsub : bv -> bv -> bv.
 
     axiom bvsubP (bv1 bv2 : bv) :
-     toint (bvsub bv1 bv2) = (toint bv1 - toint bv2) %% 2^size.
+      toint (bvsub bv1 bv2) = (toint bv1 - toint bv2) %% 2^size.
   end BVSub.
+
+  abstract theory BVMul.
+    op bvmul : bv -> bv -> bv.
+
+    axiom bvmulP (bv1 bv2 : bv) :
+      toint (bvmul bv1 bv2) = (toint bv1 * toint bv2) %% 2^size.
+  end BVMul.
+
+  abstract theory BVUDiv.
+    op bvudiv : bv -> bv -> bv.
+
+    axiom bvudivP (bv1 bv2 : bv) : toint bv2 <> 0 =>
+      toint (bvudiv bv1 bv2) = toint bv1 %/ toint bv2.
+  end BVUDiv.
+
+  abstract theory BVURem.
+    op bvurem : bv -> bv -> bv.
+
+    axiom bvuremP (bv1 bv2 : bv) :
+      toint (bvurem bv1 bv2) = toint bv1 %% toint bv2.
+  end BVURem.
+
+  abstract theory BVSHL.
+    op bvshl : bv -> bv -> bv.
+
+    axiom bvshlP (bv1 bv2 : bv) : toint (bvshl bv1 bv2) =
+      toint bv1 * 2 ^ (toint bv2).
+  end BVSHL.
+
+  abstract theory BVSHR.
+    op bvshr : bv -> bv -> bv.
+
+    axiom bvshrP (bv1 bv2 : bv) : toint (bvshr bv1 bv2) =
+      toint bv1 %/ 2 ^ (toint bv2).
+  end BVSHR.
+
+  abstract theory BVAnd.
+    op bvand : bv -> bv -> bv.
+
+    axiom bvandP (bv1 bv2 : bv) : tolist (bvand bv1 bv2) =
+      map (fun (b : _ * _) => b.`1 /\ b.`2) (zip (tolist bv1) (tolist bv2)).
+  end BVAnd.
+
+  abstract theory BVOr.
+    op bvor : bv -> bv -> bv.
+
+    axiom bvorP (bv1 bv2 : bv) : tolist (bvor bv1 bv2) =
+      map (fun (b : _ * _) => b.`1 \/ b.`2) (zip (tolist bv1) (tolist bv2)).
+  end BVOr.
+
+  abstract theory BVNot.
+    op bvnot : bv -> bv.
+
+    axiom bvnotP (bv : bv) : tolist (bvnot bv) =
+      map (fun b => !b) (tolist bv).
+  end BVNot.
 end BV.
 
 (* -------------------------------------------------------------------- *)
